src/Analysis/Instances/Sign/Sign_Call_Spec.thy
@@ -142,4 +142,115 @@ theorem sign_spec_post_fixpoint_sound_split:
         [OF pp[unfolded Sign_spec_generator_split_eq] inr inl S_sound finE finC
             cover_edge cover_comb cover_entry])
 
+subsection \<open>Stage 1D: sign through the heterogeneous generator\<close>
+
+definition sign_dg_cmb ::
+  "unit \<Rightarrow> pp \<Rightarrow> pp
+   \<Rightarrow> (pp \<times> unit, unit, (sign abs_state, sign abs_state) dg_state) strategy_tree"
+where
+  "sign_dg_cmb ctx cc ex =
+     map_gtree (\<lambda>_. ())
+       (map_ltree (\<lambda>w. (w, ctx))
+         (dg_spec_combine_tree (unit_dg_spec sign_tf) cc ex))"
+
+definition sign_dg_generator ::
+  "cfg \<Rightarrow> sign abs_state \<Rightarrow> sign abs_state
+   \<Rightarrow> (pp \<times> unit, unit, (sign abs_state, sign abs_state) dg_state) eqsT"
+where
+  "sign_dg_generator g bot0 s0 =
+     side_cfg_T_eff_cmp_seed_dg (\<lambda>_. ()) sign_dg_cmb
+       (\<lambda>_. fresh_frame_sign) g (unit_dg_spec sign_tf)
+       bot0 (restrict_local s0) (restrict_global s0)"
+
+lemma sign_dg_cmb_pack:
+  "sign_dg_cmb ctx cc ex =
+   pack_dg_tree
+     (map_gtree (\<lambda>_. ())
+       (map_ltree (\<lambda>w. (w, ctx)) (unit_combine_tree cc ex)))"
+  unfolding sign_dg_cmb_def combine_unit_dg_spec_pack
+  by (simp add: pack_dg_tree_map_ltree pack_dg_tree_map_gtree)
+
+lemma Sign_spec_cmb_unit_eq:
+  "Sign_spec.spec_cmb sign_etf_unit =
+   (\<lambda>ctx cc ex. map_gtree (\<lambda>_. ())
+     (map_ltree (\<lambda>w. (w, ctx)) (unit_combine_tree cc ex)))"
+  by (rule ext)+
+    (simp add: Sign_spec.spec_cmb_def sign_etf_unit_combine_tree)
+
+lemma Sign_spec_generator_unit_eq:
+  "Sign_spec.spec_generator g sign_etf_unit bot0 s0 =
+   side_cfg_T_eff_cmp_seed (\<lambda>_. ())
+     (\<lambda>ctx cc ex. map_gtree (\<lambda>_. ())
+       (map_ltree (\<lambda>w. (w, ctx)) (unit_combine_tree cc ex)))
+     (\<lambda>_. fresh_frame_sign) g sign_etf_unit bot0 s0"
+  by (simp add: Sign_spec.spec_generator_def Sign_spec_cmb_unit_eq)
+
+theorem sign_dg_generator_eq:
+  "sign_dg_generator g bot0 s0 =
+   (\<lambda>x. pack_dg_tree
+     (Sign_spec.spec_generator g sign_etf_unit bot0 s0 x))"
+  apply (subst Sign_spec_generator_unit_eq)
+  unfolding sign_dg_generator_def sign_etf_unit_def
+  apply (rule side_cfg_T_eff_cmp_seed_dg_unit)
+  apply (rule sign_dg_cmb_pack)
+  done
+
+corollary sign_dg_post_fixpoint_iff:
+  "part_post_solution (sign_dg_generator g bot0 s0) x (dg_env sigma) vars
+   \<longleftrightarrow>
+   part_post_solution
+     (Sign_spec.spec_generator g sign_etf_unit bot0 s0) x sigma vars"
+proof -
+  note gen = sign_dg_generator_eq
+  show ?thesis
+    unfolding gen
+    by (rule part_post_solution_pack_dg_iff)
+qed
+
+theorem sign_spec_post_fixpoint_sound_dg:
+  fixes sigma :: "pp \<times> unit + unit \<Rightarrow> sign abs_state"
+  assumes pp:
+      "part_post_solution (sign_dg_generator g bot0 s0) x (dg_env sigma) vars"
+    and inr: "inr_slot_locals_bot_ctx sigma"
+    and inl: "inl_slot_globals_bot_ctx sigma"
+    and S_sound: "S \<le> \<lbrakk>s0\<rbrakk>"
+    and finE: "finite (edges g)"
+    and finC: "finite (combines g)"
+    and cover_edge: "\<And>u a w. (u, a, w) \<in> edges g \<Longrightarrow> (w, ()) \<in> vars"
+    and cover_comb: "\<And>cc ex ret. (cc, ex, ret) \<in> combines g \<Longrightarrow> (ret, ()) \<in> vars"
+    and cover_entry: "(cfg_entry g, ()) \<in> vars"
+  shows "cfg_collect_ctx (\<lambda>_. ()) (\<lambda>_ _. True) g S v0 ()
+           \<le> \<lbrakk>side_env_cmp (\<lambda>_ _. True) sigma (v0, ())\<rbrakk>"
+proof -
+  have pp': "part_post_solution
+      (Sign_spec.spec_generator g sign_etf_unit bot0 s0) x sigma vars"
+    using pp sign_dg_post_fixpoint_iff by blast
+  show ?thesis
+    by (rule sign_spec_post_fixpoint_sound
+          [OF pp' inr inl S_sound finE finC
+              cover_edge cover_comb cover_entry])
+qed
+
+subsection \<open>Stage 1D: Retain through independent Answer and Side domains\<close>
+
+theorem sign_retain_dg_post_fixpoint_iff:
+  fixes sigma :: "pp \<times> unit + unit \<Rightarrow> sign abs_state"
+  shows
+    "part_post_solution
+       (retain_dg_generator g sign_tf fresh_frame_sign bot0 s0)
+       x (retain_hetero_rep sigma) vars
+     \<longleftrightarrow>
+     part_post_solution
+       (retain_generator g sign_tf fresh_frame_sign bot0 s0)
+       x sigma vars"
+  by (rule part_post_solution_retain_dg_iff)
+
+text \<open>
+  This instantiation uses
+  \<open>D = (sign abs_state, sign abs_state) dg_state\<close> and
+  \<open>G = sign abs_state\<close>.  The snapshot is confined to Retain's
+  \<open>D\<close>; the generator consumes only the standard \<open>dg_spec\<close>
+  interface.
+\<close>
+
 end
